LeanSAT/BitBlast/BVExpr/BitBlast/Impl/Replicate.lean
@@ -1,0 +1,40 @@
+/-
+Copyright (c) 2024 Lean FRO, LLC. All rights reserved.
+Released under Apache 2.0 license as described in the file LICENSE.
+Authors: Henrik Böving
+-/
+import LeanSAT.BitBlast.BVExpr.Basic
+import LeanSAT.AIG.LawfulStreamOperator
+
+namespace BVExpr
+namespace bitblast
+
+variable [Hashable α] [DecidableEq α]
+
+structure ReplicateTarget (aig : AIG α) (combined : Nat) where
+  {w : Nat}
+  n : Nat
+  inner : AIG.RefStream aig w
+  h : combined = w * n
+
+def blastReplicate (aig : AIG α) (target : ReplicateTarget aig newWidth)
+    : AIG.RefStreamEntry α newWidth :=
+  let ⟨n, inner, h⟩ := target
+  let ref := go n 0 (by omega) inner .empty
+  ⟨aig, h ▸ ref⟩
+where
+  go {aig : AIG α} {w : Nat} (n : Nat) (curr : Nat) (hcurr : curr ≤ n) (input : AIG.RefStream aig w)
+      (s : AIG.RefStream aig (w * curr)) : AIG.RefStream aig (w * n) :=
+    if h : curr < n then
+      let s := s.append input
+      go n (curr + 1) (by omega) input s
+    else
+      have : curr = n := by omega
+      this ▸ s
+
+instance : AIG.LawfulStreamOperator α ReplicateTarget blastReplicate where
+  le_size := by simp [blastReplicate]
+  decl_eq := by simp [blastReplicate]
+
+end bitblast
+end BVExpr
